if positive terms converge and negative terms converge
then you can take the sum of them to be 
$$\sum_{n=1}^{\infty} a_{n}^+-(a_{n}^-)=\sum_{n=1}^{\infty} a_{n}^+ - \sum_{n=1}^{\infty} a_{n}^-=\sum_{n=1}^{\infty} \lvert a_{n} \rvert $$

what is a rearrangement$\implies$
example of conditional rearrangement
why is this i.e. the infinite series thing

A rearrangement of a series $\sum_{n=1}^{\infty}a_{k}$ is a series $\sum_{n=1}^{\infty}b_{k}$ for which there is a bijection $f:\mathbb{N}\to \mathbb{N}$ such that $f_{f(k)}=a_{k}$

$$=1-\frac{1}{2}+\frac{1}{3}-\frac{1}{4}+\frac{1}{5}-\frac{1}{6}+\frac{1}{7}-\frac{1}{8}+\frac{1}{9}$$